added SIMD - wip - and passing hax

hax-driver.py
@@ -127,7 +127,7 @@ elif options.kyber_reference:
             f"-** +libcrux::kem::kyber::** +!libcrux_platform::platform::* {exclude_sha3_implementations} -libcrux::**::types::index_impls::**",
             "fstar",
             "--interfaces",
-            "+* -libcrux::kem::kyber::types +!libcrux_platform::**",
+            "+* -libcrux::kem::kyber::types +!libcrux_platform::** +!libcrux::digest::**",
         ],
         cwd=".",
         env=hax_env,
