src/kem/kyber/hash_functions.rs
@@ -1,10 +1,13 @@
 #![allow(non_snake_case)]
 
-use libcrux_platform::simd256_support;
+use digest::{Shake128State,shake128_init,shake128_absorb_final,shake128_squeeze_nblocks};
+#[cfg(simd256)]
+use digest::{Shake128StateX4,shake128_init_x4,shake128_absorb_final_x4,shake128_squeeze_nblocks_x4};
+// use libcrux_platform::simd256_support;
 
 use crate::digest::{self, digest_size, Algorithm};
 
-use super::constants::{H_DIGEST_SIZE, REJECTION_SAMPLING_SEED_SIZE};
+use super::constants::{H_DIGEST_SIZE};
 
 pub(crate) fn G(input: &[u8]) -> [u8; digest_size(Algorithm::Sha3_512)] {
     digest::sha3_512(input)
@@ -18,97 +21,98 @@ pub(crate) fn PRF<const LEN: usize>(input: &[u8]) -> [u8; LEN] {
     digest::shake256::<LEN>(input)
 }
 
+// The following API uses the repeated squeeze API
+// The first version uses Scalar SHAKE 128
+#[cfg(not(simd256))]
+pub(crate) struct XofState<const K:usize> {
+    states: [Shake128State; K]
+}
+
+#[cfg(not(simd256))]
 #[inline(always)]
-pub(crate) fn XOFx4<const K: usize>(
-    input: [[u8; 34]; K],
-) -> [[u8; REJECTION_SAMPLING_SEED_SIZE]; K] {
-    let mut out = [[0u8; REJECTION_SAMPLING_SEED_SIZE]; K];
-
-    if !simd256_support() {
-        // Without SIMD256 support we fake it and call shak128 4 times.
-        // While shak128x4 does this too, this is faster because we only do the
-        // required number of invocations (K).
-        for i in 0..K {
-            out[i] = digest::shake128::<REJECTION_SAMPLING_SEED_SIZE>(&input[i]);
-        }
-    } else {
-        // Always do 4 SHA3 at a time even if we need less.
-        // XXX: Cast for hax extraction
-        match K as u8 {
-            2 => {
-                let (d0, d1, _, _) = digest::shake128x4::<REJECTION_SAMPLING_SEED_SIZE>(
-                    &input[0], &input[1], &input[0], &input[1],
-                );
-                out[0] = d0;
-                out[1] = d1;
-            }
-            3 => {
-                let (d0, d1, d2, _) = digest::shake128x4::<REJECTION_SAMPLING_SEED_SIZE>(
-                    &input[0], &input[1], &input[2], &input[0],
-                );
-                out[0] = d0;
-                out[1] = d1;
-                out[2] = d2;
-            }
-            4 => {
-                let (d0, d1, d2, d3) = digest::shake128x4::<REJECTION_SAMPLING_SEED_SIZE>(
-                    &input[0], &input[1], &input[2], &input[3],
-                );
-                out[0] = d0;
-                out[1] = d1;
-                out[2] = d2;
-                out[3] = d3;
-            }
-            _ => unreachable!(),
-        };
+pub(crate) fn XOF_absorb<const K: usize>(input: [[u8; 34]; K]) -> XofState<K> {
+    let mut out_vec : Vec<Shake128State> = Vec::new();
+    for i in 0..K {
+        let mut st = shake128_init();
+        shake128_absorb_final(&mut st,&input[i]);
+        out_vec.push(st);
     }
+    let states:[Shake128State; K] = out_vec.try_into().unwrap_or_else(|_| panic!());
+    XofState {states}
 
+    // The following does not work with Eurydice because of "from_fn"
+    // let mut out : [Shake128State; K] = 
+    //     core::array::from_fn(|_| Shake128State::new());
+    // for i in 0..K {
+    //     out[i].absorb_final(&input[i]);
+    // }
+    // out
+}
+
+#[cfg(not(simd256))]
+#[inline(always)]
+pub(crate) fn XOF_squeeze_three_blocks<const K: usize>(
+    xof_state: &mut XofState<K>,
+) -> [[u8; 168 * 3]; K] {
+    let mut out = [[0; 168 * 3]; K];
+    for i in 0..K {
+        out[i] = shake128_squeeze_nblocks(&mut xof_state.states[i]);
+    }
+    out
+}
+
+#[cfg(not(simd256))]
+#[inline(always)]
+pub(crate) fn XOF_squeeze_block<const K: usize>(xof_state: &mut XofState<K>) -> [[u8; 168]; K] {
+    let mut out: [[u8; 168]; K] = [[0; 168]; K];
+    for i in 0..K {
+        out[i] = shake128_squeeze_nblocks(&mut xof_state.states[i]);
+    }
     out
 }
 
 // The following API uses the repeated squeeze API
-// Currently it only supports Scalar SHAKE, adapting it to SIMD SHAKE is a todo
-type XofState = crate::digest::incremental::Shake128State;
+// The second version uses SIMD256 SHAKE 128
+#[cfg(simd256)]
+type XofState<const K:usize> = X4(crate::digest::Shake128StateX4);
 
-// The following does not work with Eurydice because of "from_fn"
+#[cfg(simd256)]
 #[inline(always)]
-pub(crate) fn XOF_absorb<const K: usize>(input: [[u8; 34]; K]) -> [XofState; K] {
-    let mut out = core::array::from_fn(|_| crate::digest::incremental::Shake128State::new());
-    for i in 0..K {
-        out[i].absorb_final(&input[i]);
+pub(crate) fn XOF_absorb<const K: usize>(input: [[u8; 34]; K]) -> XofState<K> {
+    let mut out : crate::digest::Shake128StateX4 = crate::digest::Shake128StateX4::new();
+    match K {
+        2 => {out.absorb_final(input[0],input[1],input[0],input[0]);out}
+        3 => {out.absorb_final(input[0],input[1],input[2],input[0]);out}
+        4 => {out.absorb_final(input[0],input[1],input[2],input[3]);out}
+        _ => {unreachable!()}
     }
-    out
 }
 
-// The following is an experiment to avoid "from_fn" and use "map" instead
-#[inline(always)]
-pub(crate) fn XofStateAbsorb(input: [u8; 34]) -> XofState {
-    let mut out = crate::digest::incremental::Shake128State::new();
-    out.absorb_final(&input);
-    out
-} 
-
-#[inline(always)]
-pub(crate) fn XOF_absorb_map<const K: usize>(input: [[u8; 34]; K]) -> [XofState; K] {
-    input.map(XofStateAbsorb)
-}
-
+#[cfg(simd256)]
 #[inline(always)]
 pub(crate) fn XOF_squeeze_three_blocks<const K: usize>(
-    state: &mut [XofState; K],
+    state: &mut XofState<K>,
 ) -> [[u8; 168 * 3]; K] {
-    let mut out = [[0; 168 * 3]; K];
-    for i in 0..K {
-        out[i] = state[i].squeeze_nblocks();
+    let mut output = [[0; 168 * 3]; K];
+    let mut tmp = [[0; 168 * 3]; 2];
+    match K {
+        2 => {state.squeeze_nblocks(&mut output[0],&mut output[1],&mut tmp[0],&mut tmp[1]); output}
+        3 => {state.squeeze_nblocks(&mut output[0],&mut output[1],&mut output[2],&mut tmp[1]); output}
+        4 => {state.squeeze_nblocks(&mut output[0],&mut output[1],&mut output[2],&mut output[3]); output}
+        _ => {unreachable!()}
     }
-    out
 }
 
+#[cfg(simd256)]
 #[inline(always)]
-pub(crate) fn XOF_squeeze_block<const K: usize>(state: &mut [XofState; K]) -> [[u8; 168]; K] {
+pub(crate) fn XOF_squeeze_block<const K: usize>(state: &mut XofState<K>) -> [[u8; 168]; K] {
     let mut out: [[u8; 168]; K] = [[0; 168]; K];
-    for i in 0..K {
-        out[i] = state[i].squeeze_nblocks();
+    let mut tmp = [[0; 168 * 3]; 2];
+    match K {
+        2 => {state.squeeze_nblocks(&mut output[0],&mut output[1],&mut tmp[0],&mut tmp[1]); output}
+        3 => {state.squeeze_nblocks(&mut output[0],&mut output[1],&mut output[2],&mut tmp[0]); output}
+        4 => {state.squeeze_nblocks(&mut output[0],&mut output[1],&mut output[2],&mut output[3]); output}
+        _ => {unreachable!()}
     }
-    out
 }
+
