sys/hacl/src/bindings.rs
@@ -348,6 +348,44 @@ extern "C" {
         outputByteLen: u32,
     );
 }
+
+extern "C" {
+    pub fn Hacl_Hash_SHA3_Simd256_state_malloc() -> *mut Lib_IntVector_Intrinsics_vec256;
+}
+extern "C" {
+    pub fn Hacl_Hash_SHA3_Simd256_state_free(s: *mut Lib_IntVector_Intrinsics_vec256);
+}
+extern "C" {
+    pub fn Hacl_Hash_SHA3_Simd256_shake128_absorb_nblocks(
+        state: *mut Lib_IntVector_Intrinsics_vec256,
+        input0: *mut u8,
+        input1: *mut u8,
+        input2: *mut u8,
+        input3: *mut u8,
+        inputByteLen: u32,
+    );
+}
+extern "C" {
+    pub fn Hacl_Hash_SHA3_Simd256_shake128_absorb_final(
+        state: *mut Lib_IntVector_Intrinsics_vec256,
+        input0: *mut u8,
+        input1: *mut u8,
+        input2: *mut u8,
+        input3: *mut u8,
+        inputByteLen: u32,
+    );
+}
+extern "C" {
+    pub fn Hacl_Hash_SHA3_Simd256_shake128_squeeze_nblocks(
+        state: *mut Lib_IntVector_Intrinsics_vec256,
+        output0: *mut u8,
+        output1: *mut u8,
+        output2: *mut u8,
+        output3: *mut u8,
+        outputByteLen: u32,
+    );
+}
+
 extern "C" {
     pub fn Hacl_Hash_SHA3_absorb_inner(rateInBytes: u32, block: *mut u8, s: *mut u64);
 }
