proofs/fstar/extraction/Libcrux.Digest.fsti
@@ -9,23 +9,15 @@ val sha3_256_ (payload: t_Slice u8)
 val sha3_512_ (payload: t_Slice u8)
     : Prims.Pure (t_Array u8 (sz 64)) Prims.l_True (fun _ -> Prims.l_True)
 
-val shake128 (v_LEN: usize) (data: t_Slice u8)
-    : Prims.Pure (t_Array u8 v_LEN) Prims.l_True (fun _ -> Prims.l_True)
-
 val shake256 (v_LEN: usize) (data: t_Slice u8)
     : Prims.Pure (t_Array u8 v_LEN) Prims.l_True (fun _ -> Prims.l_True)
 
-val shake128x4_portable (v_LEN: usize) (data0 data1 data2 data3: t_Slice u8)
-    : Prims.Pure (t_Array u8 v_LEN & t_Array u8 v_LEN & t_Array u8 v_LEN & t_Array u8 v_LEN)
-      Prims.l_True
-      (fun _ -> Prims.l_True)
+type t_Shake128State
 
-val shake128x4_256_ (v_LEN: usize) (data0 data1 data2 data3: t_Slice u8)
-    : Prims.Pure (t_Array u8 v_LEN & t_Array u8 v_LEN & t_Array u8 v_LEN & t_Array u8 v_LEN)
-      Prims.l_True
-      (fun _ -> Prims.l_True)
+val shake128_absorb_final (st: t_Shake128State) (data: t_Slice u8)
+    : Prims.Pure t_Shake128State Prims.l_True (fun _ -> Prims.l_True)
 
-val shake128x4 (v_LEN: usize) (data0 data1 data2 data3: t_Slice u8)
-    : Prims.Pure (t_Array u8 v_LEN & t_Array u8 v_LEN & t_Array u8 v_LEN & t_Array u8 v_LEN)
-      Prims.l_True
-      (fun _ -> Prims.l_True)
+val shake128_init: Prims.unit -> Prims.Pure t_Shake128State Prims.l_True (fun _ -> Prims.l_True)
+
+val shake128_squeeze_nblocks (v_OUTPUT_BYTES: usize) (st: t_Shake128State)
+    : Prims.Pure (t_Shake128State & t_Array u8 v_OUTPUT_BYTES) Prims.l_True (fun _ -> Prims.l_True)
