proofs/fstar/extraction/Libcrux.Kem.Kyber.Hash_functions.fst
@@ -9,95 +9,128 @@ let v_H (input: t_Slice u8) = Libcrux.Digest.sha3_256_ input
 
 let v_PRF (v_LEN: usize) (input: t_Slice u8) = Libcrux.Digest.shake256 v_LEN input
 
-let v_XOFx4 (v_K: usize) (input: t_Array (t_Array u8 (sz 34)) v_K) =
-  let out:t_Array (t_Array u8 (sz 840)) v_K =
-    Rust_primitives.Hax.repeat (Rust_primitives.Hax.repeat 0uy (sz 840) <: t_Array u8 (sz 840)) v_K
+let v_XOF_absorb (v_K: usize) (input: t_Array (t_Array u8 (sz 34)) v_K) =
+  let (out_vec: Alloc.Vec.t_Vec Libcrux.Digest.t_Shake128State Alloc.Alloc.t_Global):Alloc.Vec.t_Vec
+    Libcrux.Digest.t_Shake128State Alloc.Alloc.t_Global =
+    Alloc.Vec.impl__new ()
   in
-  let out:t_Array (t_Array u8 (sz 840)) v_K =
-    if ~.(Libcrux_platform.Platform.simd256_support () <: bool)
-    then
-      Core.Iter.Traits.Iterator.f_fold (Core.Iter.Traits.Collect.f_into_iter ({
-                Core.Ops.Range.f_start = sz 0;
-                Core.Ops.Range.f_end = v_K
-              }
-              <:
-              Core.Ops.Range.t_Range usize)
-          <:
-          Core.Ops.Range.t_Range usize)
-        out
-        (fun out i ->
-            let out:t_Array (t_Array u8 (sz 840)) v_K = out in
-            let i:usize = i in
-            Rust_primitives.Hax.Monomorphized_update_at.update_at_usize out
-              i
-              (Libcrux.Digest.shake128 (sz 840)
-                  (Rust_primitives.unsize (input.[ i ] <: t_Array u8 (sz 34)) <: t_Slice u8)
-                <:
-                t_Array u8 (sz 840))
+  let out_vec:Alloc.Vec.t_Vec Libcrux.Digest.t_Shake128State Alloc.Alloc.t_Global =
+    Core.Iter.Traits.Iterator.f_fold (Core.Iter.Traits.Collect.f_into_iter ({
+              Core.Ops.Range.f_start = sz 0;
+              Core.Ops.Range.f_end = v_K
+            }
             <:
-            t_Array (t_Array u8 (sz 840)) v_K)
-    else
-      let out:t_Array (t_Array u8 (sz 840)) v_K =
-        match cast (v_K <: usize) <: u8 with
-        | 2uy ->
-          let d0, d1, _, _:(t_Array u8 (sz 840) & t_Array u8 (sz 840) & t_Array u8 (sz 840) &
-            t_Array u8 (sz 840)) =
-            Libcrux.Digest.shake128x4 (sz 840)
-              (Rust_primitives.unsize (input.[ sz 0 ] <: t_Array u8 (sz 34)) <: t_Slice u8)
-              (Rust_primitives.unsize (input.[ sz 1 ] <: t_Array u8 (sz 34)) <: t_Slice u8)
-              (Rust_primitives.unsize (input.[ sz 0 ] <: t_Array u8 (sz 34)) <: t_Slice u8)
-              (Rust_primitives.unsize (input.[ sz 1 ] <: t_Array u8 (sz 34)) <: t_Slice u8)
+            Core.Ops.Range.t_Range usize)
+        <:
+        Core.Ops.Range.t_Range usize)
+      out_vec
+      (fun out_vec i ->
+          let out_vec:Alloc.Vec.t_Vec Libcrux.Digest.t_Shake128State Alloc.Alloc.t_Global =
+            out_vec
           in
-          let out:t_Array (t_Array u8 (sz 840)) v_K =
-            Rust_primitives.Hax.Monomorphized_update_at.update_at_usize out (sz 0) d0
+          let i:usize = i in
+          let st:Libcrux.Digest.t_Shake128State = Libcrux.Digest.shake128_init () in
+          let st:Libcrux.Digest.t_Shake128State =
+            Libcrux.Digest.shake128_absorb_final st
+              (Rust_primitives.unsize (input.[ i ] <: t_Array u8 (sz 34)) <: t_Slice u8)
           in
-          let out:t_Array (t_Array u8 (sz 840)) v_K =
-            Rust_primitives.Hax.Monomorphized_update_at.update_at_usize out (sz 1) d1
+          let out_vec:Alloc.Vec.t_Vec Libcrux.Digest.t_Shake128State Alloc.Alloc.t_Global =
+            Alloc.Vec.impl_1__push out_vec st
           in
-          out
-        | 3uy ->
-          let d0, d1, d2, _:(t_Array u8 (sz 840) & t_Array u8 (sz 840) & t_Array u8 (sz 840) &
-            t_Array u8 (sz 840)) =
-            Libcrux.Digest.shake128x4 (sz 840)
-              (Rust_primitives.unsize (input.[ sz 0 ] <: t_Array u8 (sz 34)) <: t_Slice u8)
-              (Rust_primitives.unsize (input.[ sz 1 ] <: t_Array u8 (sz 34)) <: t_Slice u8)
-              (Rust_primitives.unsize (input.[ sz 2 ] <: t_Array u8 (sz 34)) <: t_Slice u8)
-              (Rust_primitives.unsize (input.[ sz 0 ] <: t_Array u8 (sz 34)) <: t_Slice u8)
-          in
-          let out:t_Array (t_Array u8 (sz 840)) v_K =
-            Rust_primitives.Hax.Monomorphized_update_at.update_at_usize out (sz 0) d0
-          in
-          let out:t_Array (t_Array u8 (sz 840)) v_K =
-            Rust_primitives.Hax.Monomorphized_update_at.update_at_usize out (sz 1) d1
-          in
-          let out:t_Array (t_Array u8 (sz 840)) v_K =
-            Rust_primitives.Hax.Monomorphized_update_at.update_at_usize out (sz 2) d2
-          in
-          out
-        | 4uy ->
-          let d0, d1, d2, d3:(t_Array u8 (sz 840) & t_Array u8 (sz 840) & t_Array u8 (sz 840) &
-            t_Array u8 (sz 840)) =
-            Libcrux.Digest.shake128x4 (sz 840)
-              (Rust_primitives.unsize (input.[ sz 0 ] <: t_Array u8 (sz 34)) <: t_Slice u8)
-              (Rust_primitives.unsize (input.[ sz 1 ] <: t_Array u8 (sz 34)) <: t_Slice u8)
-              (Rust_primitives.unsize (input.[ sz 2 ] <: t_Array u8 (sz 34)) <: t_Slice u8)
-              (Rust_primitives.unsize (input.[ sz 3 ] <: t_Array u8 (sz 34)) <: t_Slice u8)
-          in
-          let out:t_Array (t_Array u8 (sz 840)) v_K =
-            Rust_primitives.Hax.Monomorphized_update_at.update_at_usize out (sz 0) d0
-          in
-          let out:t_Array (t_Array u8 (sz 840)) v_K =
-            Rust_primitives.Hax.Monomorphized_update_at.update_at_usize out (sz 1) d1
-          in
-          let out:t_Array (t_Array u8 (sz 840)) v_K =
-            Rust_primitives.Hax.Monomorphized_update_at.update_at_usize out (sz 2) d2
-          in
-          let out:t_Array (t_Array u8 (sz 840)) v_K =
-            Rust_primitives.Hax.Monomorphized_update_at.update_at_usize out (sz 3) d3
-          in
-          out
-        | _ -> out
-      in
-      out
+          out_vec)
   in
-  out
+  let (states: t_Array Libcrux.Digest.t_Shake128State v_K):t_Array Libcrux.Digest.t_Shake128State
+    v_K =
+    Core.Result.impl__unwrap_or_else (Core.Convert.f_try_into out_vec
+        <:
+        Core.Result.t_Result (t_Array Libcrux.Digest.t_Shake128State v_K)
+          (Alloc.Vec.t_Vec Libcrux.Digest.t_Shake128State Alloc.Alloc.t_Global))
+      (fun temp_0_ ->
+          let _:Alloc.Vec.t_Vec Libcrux.Digest.t_Shake128State Alloc.Alloc.t_Global = temp_0_ in
+          Rust_primitives.Hax.never_to_any (Core.Panicking.panic "explicit panic"
+              <:
+              Rust_primitives.Hax.t_Never)
+          <:
+          t_Array Libcrux.Digest.t_Shake128State v_K)
+  in
+  { f_states = states } <: t_XofState v_K
+
+let v_XOF_squeeze_block (v_K: usize) (xof_state: t_XofState v_K) =
+  let (out: t_Array (t_Array u8 (sz 168)) v_K):t_Array (t_Array u8 (sz 168)) v_K =
+    Rust_primitives.Hax.repeat (Rust_primitives.Hax.repeat 0uy (sz 168) <: t_Array u8 (sz 168)) v_K
+  in
+  let out, xof_state:(t_Array (t_Array u8 (sz 168)) v_K & t_XofState v_K) =
+    Core.Iter.Traits.Iterator.f_fold (Core.Iter.Traits.Collect.f_into_iter ({
+              Core.Ops.Range.f_start = sz 0;
+              Core.Ops.Range.f_end = v_K
+            }
+            <:
+            Core.Ops.Range.t_Range usize)
+        <:
+        Core.Ops.Range.t_Range usize)
+      (out, xof_state <: (t_Array (t_Array u8 (sz 168)) v_K & t_XofState v_K))
+      (fun temp_0_ i ->
+          let out, xof_state:(t_Array (t_Array u8 (sz 168)) v_K & t_XofState v_K) = temp_0_ in
+          let i:usize = i in
+          let tmp0, out:(Libcrux.Digest.t_Shake128State & t_Array u8 (sz 168)) =
+            Libcrux.Digest.shake128_squeeze_nblocks (sz 168)
+              (xof_state.f_states.[ i ] <: Libcrux.Digest.t_Shake128State)
+          in
+          let xof_state:t_XofState v_K =
+            {
+              xof_state with
+              f_states
+              =
+              Rust_primitives.Hax.Monomorphized_update_at.update_at_usize xof_state.f_states i tmp0
+            }
+            <:
+            t_XofState v_K
+          in
+          let hoist21:t_Array u8 (sz 168) = out in
+          let hoist22:t_Array (t_Array u8 (sz 168)) v_K =
+            Rust_primitives.Hax.Monomorphized_update_at.update_at_usize out i hoist21
+          in
+          hoist22, xof_state <: (t_Array (t_Array u8 (sz 168)) v_K & t_XofState v_K))
+  in
+  let hax_temp_output:t_Array (t_Array u8 (sz 168)) v_K = out in
+  xof_state, hax_temp_output <: (t_XofState v_K & t_Array (t_Array u8 (sz 168)) v_K)
+
+let v_XOF_squeeze_three_blocks (v_K: usize) (xof_state: t_XofState v_K) =
+  let out:t_Array (t_Array u8 (sz 504)) v_K =
+    Rust_primitives.Hax.repeat (Rust_primitives.Hax.repeat 0uy (sz 504) <: t_Array u8 (sz 504)) v_K
+  in
+  let out, xof_state:(t_Array (t_Array u8 (sz 504)) v_K & t_XofState v_K) =
+    Core.Iter.Traits.Iterator.f_fold (Core.Iter.Traits.Collect.f_into_iter ({
+              Core.Ops.Range.f_start = sz 0;
+              Core.Ops.Range.f_end = v_K
+            }
+            <:
+            Core.Ops.Range.t_Range usize)
+        <:
+        Core.Ops.Range.t_Range usize)
+      (out, xof_state <: (t_Array (t_Array u8 (sz 504)) v_K & t_XofState v_K))
+      (fun temp_0_ i ->
+          let out, xof_state:(t_Array (t_Array u8 (sz 504)) v_K & t_XofState v_K) = temp_0_ in
+          let i:usize = i in
+          let tmp0, out:(Libcrux.Digest.t_Shake128State & t_Array u8 (sz 504)) =
+            Libcrux.Digest.shake128_squeeze_nblocks (sz 504)
+              (xof_state.f_states.[ i ] <: Libcrux.Digest.t_Shake128State)
+          in
+          let xof_state:t_XofState v_K =
+            {
+              xof_state with
+              f_states
+              =
+              Rust_primitives.Hax.Monomorphized_update_at.update_at_usize xof_state.f_states i tmp0
+            }
+            <:
+            t_XofState v_K
+          in
+          let hoist23:t_Array u8 (sz 504) = out in
+          let hoist24:t_Array (t_Array u8 (sz 504)) v_K =
+            Rust_primitives.Hax.Monomorphized_update_at.update_at_usize out i hoist23
+          in
+          hoist24, xof_state <: (t_Array (t_Array u8 (sz 504)) v_K & t_XofState v_K))
+  in
+  let hax_temp_output:t_Array (t_Array u8 (sz 504)) v_K = out in
+  xof_state, hax_temp_output <: (t_XofState v_K & t_Array (t_Array u8 (sz 504)) v_K)
