proofs/fstar/extraction/Libcrux.Kem.Kyber.Hash_functions.fsti
@@ -10,5 +10,17 @@ val v_H (input: t_Slice u8) : Prims.Pure (t_Array u8 (sz 32)) Prims.l_True (fun 
 val v_PRF (v_LEN: usize) (input: t_Slice u8)
     : Prims.Pure (t_Array u8 v_LEN) Prims.l_True (fun _ -> Prims.l_True)
 
-val v_XOFx4 (v_K: usize) (input: t_Array (t_Array u8 (sz 34)) v_K)
-    : Prims.Pure (t_Array (t_Array u8 (sz 840)) v_K) Prims.l_True (fun _ -> Prims.l_True)
+type t_XofState (v_K: usize) = { f_states:t_Array Libcrux.Digest.t_Shake128State v_K }
+
+val v_XOF_absorb (v_K: usize) (input: t_Array (t_Array u8 (sz 34)) v_K)
+    : Prims.Pure (t_XofState v_K) Prims.l_True (fun _ -> Prims.l_True)
+
+val v_XOF_squeeze_block (v_K: usize) (xof_state: t_XofState v_K)
+    : Prims.Pure (t_XofState v_K & t_Array (t_Array u8 (sz 168)) v_K)
+      Prims.l_True
+      (fun _ -> Prims.l_True)
+
+val v_XOF_squeeze_three_blocks (v_K: usize) (xof_state: t_XofState v_K)
+    : Prims.Pure (t_XofState v_K & t_Array (t_Array u8 (sz 504)) v_K)
+      Prims.l_True
+      (fun _ -> Prims.l_True)
