proofs/fstar/extraction/Libcrux.Kem.Kyber.Ind_cpa.fst
@@ -334,92 +334,6 @@ let decrypt
   in
   Libcrux.Kem.Kyber.Serialize.compress_then_serialize_message message
 
-let encrypt
-      (v_K v_CIPHERTEXT_SIZE v_T_AS_NTT_ENCODED_SIZE v_C1_LEN v_C2_LEN v_U_COMPRESSION_FACTOR v_V_COMPRESSION_FACTOR v_BLOCK_LEN v_ETA1 v_ETA1_RANDOMNESS_SIZE v_ETA2 v_ETA2_RANDOMNESS_SIZE:
-          usize)
-      (public_key: t_Slice u8)
-      (message: t_Array u8 (sz 32))
-      (randomness: t_Slice u8)
-     =
-  let tt_as_ntt:t_Array Libcrux.Kem.Kyber.Arithmetic.t_PolynomialRingElement v_K =
-    deserialize_public_key v_K
-      (public_key.[ { Core.Ops.Range.f_end = v_T_AS_NTT_ENCODED_SIZE }
-          <:
-          Core.Ops.Range.t_RangeTo usize ]
-        <:
-        t_Slice u8)
-  in
-  let seed:t_Slice u8 =
-    public_key.[ { Core.Ops.Range.f_start = v_T_AS_NTT_ENCODED_SIZE }
-      <:
-      Core.Ops.Range.t_RangeFrom usize ]
-  in
-  let v_A_transpose:t_Array (t_Array Libcrux.Kem.Kyber.Arithmetic.t_PolynomialRingElement v_K) v_K =
-    Libcrux.Kem.Kyber.Matrix.sample_matrix_A v_K
-      (into_padded_array (sz 34) seed <: t_Array u8 (sz 34))
-      false
-  in
-  let (prf_input: t_Array u8 (sz 33)):t_Array u8 (sz 33) = into_padded_array (sz 33) randomness in
-  let r_as_ntt, domain_separator:(t_Array Libcrux.Kem.Kyber.Arithmetic.t_PolynomialRingElement v_K &
-    u8) =
-    sample_vector_cbd_then_ntt v_K v_ETA1 v_ETA1_RANDOMNESS_SIZE prf_input 0uy
-  in
-  let tmp0, tmp1, out:(t_Array u8 (sz 33) & u8 &
-    t_Array Libcrux.Kem.Kyber.Arithmetic.t_PolynomialRingElement v_K) =
-    sample_ring_element_cbd v_K v_ETA2_RANDOMNESS_SIZE v_ETA2 prf_input domain_separator
-  in
-  let prf_input:t_Array u8 (sz 33) = tmp0 in
-  let domain_separator:u8 = tmp1 in
-  let error_1_:t_Array Libcrux.Kem.Kyber.Arithmetic.t_PolynomialRingElement v_K = out in
-  let prf_input:t_Array u8 (sz 33) =
-    Rust_primitives.Hax.Monomorphized_update_at.update_at_usize prf_input (sz 32) domain_separator
-  in
-  let (prf_output: t_Array u8 v_ETA2_RANDOMNESS_SIZE):t_Array u8 v_ETA2_RANDOMNESS_SIZE =
-    Libcrux.Kem.Kyber.Hash_functions.v_PRF v_ETA2_RANDOMNESS_SIZE
-      (Rust_primitives.unsize prf_input <: t_Slice u8)
-  in
-  let error_2_:Libcrux.Kem.Kyber.Arithmetic.t_PolynomialRingElement =
-    Libcrux.Kem.Kyber.Sampling.sample_from_binomial_distribution v_ETA2
-      (Rust_primitives.unsize prf_output <: t_Slice u8)
-  in
-  let u:t_Array Libcrux.Kem.Kyber.Arithmetic.t_PolynomialRingElement v_K =
-    Libcrux.Kem.Kyber.Matrix.compute_vector_u v_K v_A_transpose r_as_ntt error_1_
-  in
-  let message_as_ring_element:Libcrux.Kem.Kyber.Arithmetic.t_PolynomialRingElement =
-    Libcrux.Kem.Kyber.Serialize.deserialize_then_decompress_message message
-  in
-  let v:Libcrux.Kem.Kyber.Arithmetic.t_PolynomialRingElement =
-    Libcrux.Kem.Kyber.Matrix.compute_ring_element_v v_K
-      tt_as_ntt
-      r_as_ntt
-      error_2_
-      message_as_ring_element
-  in
-  let c1:t_Array u8 v_C1_LEN =
-    compress_then_serialize_u v_K v_C1_LEN v_U_COMPRESSION_FACTOR v_BLOCK_LEN u
-  in
-  let c2:t_Array u8 v_C2_LEN =
-    Libcrux.Kem.Kyber.Serialize.compress_then_serialize_ring_element_v v_V_COMPRESSION_FACTOR
-      v_C2_LEN
-      v
-  in
-  let (ciphertext: t_Array u8 v_CIPHERTEXT_SIZE):t_Array u8 v_CIPHERTEXT_SIZE =
-    into_padded_array v_CIPHERTEXT_SIZE (Rust_primitives.unsize c1 <: t_Slice u8)
-  in
-  let ciphertext:t_Array u8 v_CIPHERTEXT_SIZE =
-    Rust_primitives.Hax.Monomorphized_update_at.update_at_range_from ciphertext
-      ({ Core.Ops.Range.f_start = v_C1_LEN } <: Core.Ops.Range.t_RangeFrom usize)
-      (Core.Slice.impl__copy_from_slice (ciphertext.[ { Core.Ops.Range.f_start = v_C1_LEN }
-              <:
-              Core.Ops.Range.t_RangeFrom usize ]
-            <:
-            t_Slice u8)
-          (Core.Array.impl_23__as_slice v_C2_LEN c2 <: t_Slice u8)
-        <:
-        t_Slice u8)
-  in
-  ciphertext
-
 let serialize_secret_key
       (v_K v_OUT_LEN: usize)
       (key: t_Array Libcrux.Kem.Kyber.Arithmetic.t_PolynomialRingElement v_K)
@@ -528,6 +442,92 @@ let serialize_public_key
         t_Slice u8)
   in
   public_key_serialized
+
+let encrypt
+      (v_K v_CIPHERTEXT_SIZE v_T_AS_NTT_ENCODED_SIZE v_C1_LEN v_C2_LEN v_U_COMPRESSION_FACTOR v_V_COMPRESSION_FACTOR v_BLOCK_LEN v_ETA1 v_ETA1_RANDOMNESS_SIZE v_ETA2 v_ETA2_RANDOMNESS_SIZE:
+          usize)
+      (public_key: t_Slice u8)
+      (message: t_Array u8 (sz 32))
+      (randomness: t_Slice u8)
+     =
+  let tt_as_ntt:t_Array Libcrux.Kem.Kyber.Arithmetic.t_PolynomialRingElement v_K =
+    deserialize_public_key v_K
+      (public_key.[ { Core.Ops.Range.f_end = v_T_AS_NTT_ENCODED_SIZE }
+          <:
+          Core.Ops.Range.t_RangeTo usize ]
+        <:
+        t_Slice u8)
+  in
+  let seed:t_Slice u8 =
+    public_key.[ { Core.Ops.Range.f_start = v_T_AS_NTT_ENCODED_SIZE }
+      <:
+      Core.Ops.Range.t_RangeFrom usize ]
+  in
+  let v_A_transpose:t_Array (t_Array Libcrux.Kem.Kyber.Arithmetic.t_PolynomialRingElement v_K) v_K =
+    Libcrux.Kem.Kyber.Matrix.sample_matrix_A v_K
+      (into_padded_array (sz 34) seed <: t_Array u8 (sz 34))
+      false
+  in
+  let (prf_input: t_Array u8 (sz 33)):t_Array u8 (sz 33) = into_padded_array (sz 33) randomness in
+  let r_as_ntt, domain_separator:(t_Array Libcrux.Kem.Kyber.Arithmetic.t_PolynomialRingElement v_K &
+    u8) =
+    sample_vector_cbd_then_ntt v_K v_ETA1 v_ETA1_RANDOMNESS_SIZE prf_input 0uy
+  in
+  let tmp0, tmp1, out:(t_Array u8 (sz 33) & u8 &
+    t_Array Libcrux.Kem.Kyber.Arithmetic.t_PolynomialRingElement v_K) =
+    sample_ring_element_cbd v_K v_ETA2_RANDOMNESS_SIZE v_ETA2 prf_input domain_separator
+  in
+  let prf_input:t_Array u8 (sz 33) = tmp0 in
+  let domain_separator:u8 = tmp1 in
+  let error_1_:t_Array Libcrux.Kem.Kyber.Arithmetic.t_PolynomialRingElement v_K = out in
+  let prf_input:t_Array u8 (sz 33) =
+    Rust_primitives.Hax.Monomorphized_update_at.update_at_usize prf_input (sz 32) domain_separator
+  in
+  let (prf_output: t_Array u8 v_ETA2_RANDOMNESS_SIZE):t_Array u8 v_ETA2_RANDOMNESS_SIZE =
+    Libcrux.Kem.Kyber.Hash_functions.v_PRF v_ETA2_RANDOMNESS_SIZE
+      (Rust_primitives.unsize prf_input <: t_Slice u8)
+  in
+  let error_2_:Libcrux.Kem.Kyber.Arithmetic.t_PolynomialRingElement =
+    Libcrux.Kem.Kyber.Sampling.sample_from_binomial_distribution v_ETA2
+      (Rust_primitives.unsize prf_output <: t_Slice u8)
+  in
+  let u:t_Array Libcrux.Kem.Kyber.Arithmetic.t_PolynomialRingElement v_K =
+    Libcrux.Kem.Kyber.Matrix.compute_vector_u v_K v_A_transpose r_as_ntt error_1_
+  in
+  let message_as_ring_element:Libcrux.Kem.Kyber.Arithmetic.t_PolynomialRingElement =
+    Libcrux.Kem.Kyber.Serialize.deserialize_then_decompress_message message
+  in
+  let v:Libcrux.Kem.Kyber.Arithmetic.t_PolynomialRingElement =
+    Libcrux.Kem.Kyber.Matrix.compute_ring_element_v v_K
+      tt_as_ntt
+      r_as_ntt
+      error_2_
+      message_as_ring_element
+  in
+  let c1:t_Array u8 v_C1_LEN =
+    compress_then_serialize_u v_K v_C1_LEN v_U_COMPRESSION_FACTOR v_BLOCK_LEN u
+  in
+  let c2:t_Array u8 v_C2_LEN =
+    Libcrux.Kem.Kyber.Serialize.compress_then_serialize_ring_element_v v_V_COMPRESSION_FACTOR
+      v_C2_LEN
+      v
+  in
+  let (ciphertext: t_Array u8 v_CIPHERTEXT_SIZE):t_Array u8 v_CIPHERTEXT_SIZE =
+    into_padded_array v_CIPHERTEXT_SIZE (Rust_primitives.unsize c1 <: t_Slice u8)
+  in
+  let ciphertext:t_Array u8 v_CIPHERTEXT_SIZE =
+    Rust_primitives.Hax.Monomorphized_update_at.update_at_range_from ciphertext
+      ({ Core.Ops.Range.f_start = v_C1_LEN } <: Core.Ops.Range.t_RangeFrom usize)
+      (Core.Slice.impl__copy_from_slice (ciphertext.[ { Core.Ops.Range.f_start = v_C1_LEN }
+              <:
+              Core.Ops.Range.t_RangeFrom usize ]
+            <:
+            t_Slice u8)
+          (Core.Array.impl_23__as_slice v_C2_LEN c2 <: t_Slice u8)
+        <:
+        t_Slice u8)
+  in
+  ciphertext
 
 let generate_keypair
       (v_K v_PRIVATE_KEY_SIZE v_PUBLIC_KEY_SIZE v_RANKED_BYTES_PER_RING_ELEMENT v_ETA1 v_ETA1_RANDOMNESS_SIZE:
