proofs/fstar/extraction/Libcrux.Kem.Kyber.Kyber1024.fst
@@ -3,20 +3,6 @@ module Libcrux.Kem.Kyber.Kyber1024
 open Core
 open FStar.Mul
 
-let decapsulate
-      (secret_key: Libcrux.Kem.Kyber.Types.t_MlKemPrivateKey (sz 3168))
-      (ciphertext: Libcrux.Kem.Kyber.Types.t_MlKemCiphertext (sz 1568))
-     =
-  Libcrux.Kem.Kyber.decapsulate (sz 4) (sz 3168) (sz 1536) (sz 1568) (sz 1568) (sz 1536) (sz 1408)
-    (sz 160) (sz 11) (sz 5) (sz 352) (sz 2) (sz 128) (sz 2) (sz 128) (sz 1600) secret_key ciphertext
-
-let encapsulate
-      (public_key: Libcrux.Kem.Kyber.Types.t_MlKemPublicKey (sz 1568))
-      (randomness: t_Array u8 (sz 32))
-     =
-  Libcrux.Kem.Kyber.encapsulate (sz 4) (sz 1568) (sz 1568) (sz 1536) (sz 1408) (sz 160) (sz 11)
-    (sz 5) (sz 352) (sz 2) (sz 128) (sz 2) (sz 128) public_key randomness
-
 let validate_public_key (public_key: Libcrux.Kem.Kyber.Types.t_MlKemPublicKey (sz 1568)) =
   if
     Libcrux.Kem.Kyber.validate_public_key (sz 4)
@@ -31,6 +17,20 @@ let validate_public_key (public_key: Libcrux.Kem.Kyber.Types.t_MlKemPublicKey (s
     Core.Option.Option_None
     <:
     Core.Option.t_Option (Libcrux.Kem.Kyber.Types.t_MlKemPublicKey (sz 1568))
+
+let decapsulate
+      (secret_key: Libcrux.Kem.Kyber.Types.t_MlKemPrivateKey (sz 3168))
+      (ciphertext: Libcrux.Kem.Kyber.Types.t_MlKemCiphertext (sz 1568))
+     =
+  Libcrux.Kem.Kyber.decapsulate (sz 4) (sz 3168) (sz 1536) (sz 1568) (sz 1568) (sz 1536) (sz 1408)
+    (sz 160) (sz 11) (sz 5) (sz 352) (sz 2) (sz 128) (sz 2) (sz 128) (sz 1600) secret_key ciphertext
+
+let encapsulate
+      (public_key: Libcrux.Kem.Kyber.Types.t_MlKemPublicKey (sz 1568))
+      (randomness: t_Array u8 (sz 32))
+     =
+  Libcrux.Kem.Kyber.encapsulate (sz 4) (sz 1568) (sz 1568) (sz 1536) (sz 1408) (sz 160) (sz 11)
+    (sz 5) (sz 352) (sz 2) (sz 128) (sz 2) (sz 128) public_key randomness
 
 let generate_key_pair (randomness: t_Array u8 (sz 64)) =
   Libcrux.Kem.Kyber.generate_keypair (sz 4)
