proofs/fstar/extraction/Libcrux.Kem.Kyber.fst
@@ -108,6 +108,31 @@ let serialize_kem_secret_key
   in
   out
 
+let validate_public_key
+      (v_K v_RANKED_BYTES_PER_RING_ELEMENT v_PUBLIC_KEY_SIZE: usize)
+      (public_key: t_Array u8 v_PUBLIC_KEY_SIZE)
+     =
+  let pk:t_Array Libcrux.Kem.Kyber.Arithmetic.t_PolynomialRingElement v_K =
+    Libcrux.Kem.Kyber.Ind_cpa.deserialize_public_key v_K
+      (public_key.[ { Core.Ops.Range.f_end = v_RANKED_BYTES_PER_RING_ELEMENT }
+          <:
+          Core.Ops.Range.t_RangeTo usize ]
+        <:
+        t_Slice u8)
+  in
+  let public_key_serialized:t_Array u8 v_PUBLIC_KEY_SIZE =
+    Libcrux.Kem.Kyber.Ind_cpa.serialize_public_key v_K
+      v_RANKED_BYTES_PER_RING_ELEMENT
+      v_PUBLIC_KEY_SIZE
+      pk
+      (public_key.[ { Core.Ops.Range.f_start = v_RANKED_BYTES_PER_RING_ELEMENT }
+          <:
+          Core.Ops.Range.t_RangeFrom usize ]
+        <:
+        t_Slice u8)
+  in
+  public_key =. public_key_serialized
+
 let decapsulate
       (v_K v_SECRET_KEY_SIZE v_CPA_SECRET_KEY_SIZE v_PUBLIC_KEY_SIZE v_CIPHERTEXT_SIZE v_T_AS_NTT_ENCODED_SIZE v_C1_SIZE v_C2_SIZE v_VECTOR_U_COMPRESSION_FACTOR v_VECTOR_V_COMPRESSION_FACTOR v_C1_BLOCK_SIZE v_ETA1 v_ETA1_RANDOMNESS_SIZE v_ETA2 v_ETA2_RANDOMNESS_SIZE v_IMPLICIT_REJECTION_HASH_INPUT_SIZE:
           usize)
@@ -263,31 +288,6 @@ let encapsulate
   Core.Convert.f_into ciphertext, shared_secret
   <:
   (Libcrux.Kem.Kyber.Types.t_MlKemCiphertext v_CIPHERTEXT_SIZE & t_Array u8 (sz 32))
-
-let validate_public_key
-      (v_K v_RANKED_BYTES_PER_RING_ELEMENT v_PUBLIC_KEY_SIZE: usize)
-      (public_key: t_Array u8 v_PUBLIC_KEY_SIZE)
-     =
-  let pk:t_Array Libcrux.Kem.Kyber.Arithmetic.t_PolynomialRingElement v_K =
-    Libcrux.Kem.Kyber.Ind_cpa.deserialize_public_key v_K
-      (public_key.[ { Core.Ops.Range.f_end = v_RANKED_BYTES_PER_RING_ELEMENT }
-          <:
-          Core.Ops.Range.t_RangeTo usize ]
-        <:
-        t_Slice u8)
-  in
-  let public_key_serialized:t_Array u8 v_PUBLIC_KEY_SIZE =
-    Libcrux.Kem.Kyber.Ind_cpa.serialize_public_key v_K
-      v_RANKED_BYTES_PER_RING_ELEMENT
-      v_PUBLIC_KEY_SIZE
-      pk
-      (public_key.[ { Core.Ops.Range.f_start = v_RANKED_BYTES_PER_RING_ELEMENT }
-          <:
-          Core.Ops.Range.t_RangeFrom usize ]
-        <:
-        t_Slice u8)
-  in
-  public_key =. public_key_serialized
 
 let generate_keypair
       (v_K v_CPA_PRIVATE_KEY_SIZE v_PRIVATE_KEY_SIZE v_PUBLIC_KEY_SIZE v_BYTES_PER_RING_ELEMENT v_ETA1 v_ETA1_RANDOMNESS_SIZE:
